finset [subset, proper, union, diff, intersection]

theories/NewFSet.ec
@@ -1,4 +1,5 @@
 (* -------------------------------------------------------------------- *)
+require import Pred.
 require import NewList.
 
 (* -------------------------------------------------------------------- *)
@@ -18,27 +19,67 @@ lemma uniq_elems (s : 'a fset): uniq (elems s).
 proof. admit. qed.
 
 (* -------------------------------------------------------------------- *)
+op card ['a] (s : 'a fset) = size (elems s) axiomatized by cardE.
+
+(* -------------------------------------------------------------------- *)
 op mem ['a] (s : 'a fset) (x : 'a) = mem (elems s) x
   axiomatized by memE.
 
 lemma mem_oflist (s : 'a list):
   forall x, mem (oflist s) x <=> mem s x.
 proof.
-  intros=> x; rewrite !memE /= (perm_eq_mem _ (undup s)).
+  move=> x; rewrite !memE /= (perm_eq_mem _ (undup s)).
     by rewrite perm_eq_sym oflistK.
   by rewrite mem_undup.
 qed.
 
-(* -------------------------------------------------------------------- *)
-op fset0 ['a] = oflist [<:'a>] axiomatized by fset0E.
-op fset1 ['a] (z : 'a) = oflist [z] axiomatized by fset1E.
-
-op fsetD ['a] (s1 s2 : 'a fset) = oflist (elems s1 ++ elems s2)
-  axiomatized by fsetDE.
+lemma setP (s1 s2 : 'a fset):
+  (s1 = s2) <=> (forall x, mem s1 x <=> mem s2 x).
+proof. split => [-> // |]. admit. qed.
 
 (* -------------------------------------------------------------------- *)
-lemma mem_fset0: forall x, mem fset0<:'a> x <=> false.
-proof. by intros=> x; rewrite fset0E mem_oflist. qed.
+op set0 ['a] = oflist [<:'a>] axiomatized by set0E.
+op set1 ['a] (z : 'a) = oflist [z] axiomatized by set1E.
 
-lemma mem_fset1 z: forall x, mem (fset1<:'a> z) x <=> x = z.
-proof. by intros=> x; rewrite fset1E /= mem_oflist. qed.
+op setU ['a] (s1 s2 : 'a fset) = oflist (elems s1 ++ elems s2)
+  axiomatized by setUE.
+
+op setI ['a] (s1 s2 : 'a fset) = oflist (filter (mem s2) (elems s1))
+  axiomatized by setIE.
+
+op setD ['a] (s1 s2 : 'a fset) = oflist (filter (predC (mem s2)) (elems s1))
+  axiomatized by setDE.
+
+(* -------------------------------------------------------------------- *)
+lemma in_set0: forall x, mem set0<:'a> x <=> false.
+proof. by move=> x; rewrite set0E mem_oflist. qed.
+
+lemma in_set1 z: forall x, mem (set1<:'a> z) x <=> x = z.
+proof. by move=> x; rewrite set1E /= mem_oflist. qed.
+
+lemma in_setU (s1 s2 : 'a fset):
+  forall x, mem (setU s1 s2) x <=> mem s1 x \/ mem s2 x.
+proof. by move=> x; rewrite setUE /= mem_oflist mem_cat memE. qed.
+
+lemma in_setI (s1 s2 : 'a fset):
+  forall x, mem (setI s1 s2) x <=> mem s1 x /\ mem s2 x.
+proof. by move=> x; rewrite setIE /= mem_oflist mem_filter memE. qed.
+
+lemma in_setD (s1 s2 : 'a fset):
+  forall x, mem (setD s1 s2) x <=> mem s1 x /\ !mem s2 x.
+proof. by move=> x; rewrite setDE /= mem_oflist mem_filter memE. qed.
+
+(* -------------------------------------------------------------------- *)
+pred (<=) (s1 s2 : 'a fset) = mem s1 <= mem s2.
+pred (< ) (s1 s2 : 'a fset) = mem s1 <  mem s2.
+
+lemma nosmt subsetE (s1 s2 : 'a fset):
+  (s1 <= s2) <=> (mem s1 <= mem s2).
+proof. by []. qed.
+
+(* -------------------------------------------------------------------- *)
+lemma nosmt eqEsubset (A B : 'a fset) : (A = B) <=> (A <= B) /\ (B <= A).
+proof.
+  (* FIX: subpred_eqP => should from [(mem A) (mem B)] by matching *)
+  by rewrite setP !subsetE; rewrite (subpred_eqP (mem A) (mem B)).
+qed.
